disk-betree/BetreeBlockCacheSystemCrashSafeBetreeRefinement.dfy
@@ -8,6 +8,7 @@ abstract module BetreeBlockCacheSystemCrashSafeBetreeRefinement {
   import opened Maps
   import opened Sequences
   import opened BetreeSpec`Spec
+  import CrashTypes
 
   import G = BetreeGraph
   import BBCS = BetreeBlockCacheSystem
@@ -23,7 +24,7 @@ abstract module BetreeBlockCacheSystemCrashSafeBetreeRefinement {
 
   type DiskOp = M.DiskOp
   type Reference = G.Reference
-  type UIOp = BT.UIOp
+  type CrashableUIOp = BBCS.CrashableUIOp
 
   function Ik(k: BBCS.Constants) : CSBT.Constants {
     BT.Constants(BI.Constants())
@@ -46,12 +47,12 @@ abstract module BetreeBlockCacheSystemCrashSafeBetreeRefinement {
   // Right now the BlockCacheSystem assumes any valid disk
   // whereas the Betree requires the Betree to start empty
 
-  lemma RefinesBetreeMoveStep(k: BBCS.Constants, s: BBCS.Variables, s': BBCS.Variables, uiop: UIOp, dop: DiskOp, betreeStep: BetreeStep)
+  lemma RefinesBetreeMoveStep(k: BBCS.Constants, s: BBCS.Variables, s': BBCS.Variables, uiop: M.UIOp, dop: DiskOp, betreeStep: BetreeStep)
   requires BBCS.Inv(k, s)
   requires BBCS.Inv(k, s')
   requires M.BetreeMove(k.machine, s.machine, s'.machine, uiop, dop, betreeStep)
   requires D.Next(k.disk, s.disk, s'.disk, dop)
-  ensures CSBT.Next(Ik(k), I(k, s), I(k, s'), uiop)
+  ensures CSBT.Next(Ik(k), I(k, s), I(k, s'), CrashTypes.NormalOp(uiop))
   {
     assert s.machine.Ready?;
 
@@ -65,45 +66,45 @@ abstract module BetreeBlockCacheSystemCrashSafeBetreeRefinement {
 
     assert I(k, s).persistent == I(k, s').persistent;
     assert BT.NextStep(Ik(k), I(k, s).ephemeral, I(k, s').ephemeral, uiop, BT.BetreeStep(betreeStep));
-    assert CSBT.NextStep(Ik(k), I(k, s), I(k, s'), uiop, CSBT.EphemeralMoveStep);
+    assert CSBT.NextStep(Ik(k), I(k, s), I(k, s'), CrashTypes.NormalOp(uiop), CSBT.EphemeralMoveStep);
   }
 
   // TODO I suspect a lot of the below handling of BlockCache operations
   // can be reduced to stuff in the general
   // BlockCacheSystem -> CrashSafeBlockInterface proof.
 
-  lemma RefinesWriteBackStep(k: BBCS.Constants, s: BBCS.Variables, s': BBCS.Variables, uiop: UIOp, dop: DiskOp, ref: Reference)
+  lemma RefinesWriteBackStep(k: BBCS.Constants, s: BBCS.Variables, s': BBCS.Variables, uiop: M.UIOp, dop: DiskOp, ref: Reference)
   requires BBCS.Inv(k, s)
   requires BBCS.Inv(k, s')
   requires uiop.NoOp?
   requires BC.WriteBack(k.machine, s.machine, s'.machine, dop, ref)
   requires D.Write(k.disk, s.disk, s'.disk, dop);
-  ensures CSBT.Next(Ik(k), I(k, s), I(k, s'), uiop)
+  ensures CSBT.Next(Ik(k), I(k, s), I(k, s'), CrashTypes.NormalOp(uiop))
   {
     BCS.WriteBackStepPreservesGraphs(k, s, s', dop, ref);
     assert BT.NextStep(Ik(k), I(k, s).ephemeral, I(k, s').ephemeral, uiop, BT.StutterStep);
-    assert CSBT.NextStep(Ik(k), I(k, s), I(k, s'), uiop, CSBT.EphemeralMoveStep);
+    assert CSBT.NextStep(Ik(k), I(k, s), I(k, s'), CrashTypes.NormalOp(uiop), CSBT.EphemeralMoveStep);
   }
 
-  lemma RefinesWriteBackSuperblockStep(k: BBCS.Constants, s: BBCS.Variables, s': BBCS.Variables, uiop: UIOp, dop: DiskOp)
+  lemma RefinesWriteBackSuperblockStep(k: BBCS.Constants, s: BBCS.Variables, s': BBCS.Variables, uiop: M.UIOp, dop: DiskOp)
   requires BBCS.Inv(k, s)
   requires BBCS.Inv(k, s')
   requires uiop.NoOp?
   requires BC.WriteBackSuperblock(k.machine, s.machine, s'.machine, dop)
   requires D.Write(k.disk, s.disk, s'.disk, dop);
-  ensures CSBT.Next(Ik(k), I(k, s), I(k, s'), uiop)
+  ensures CSBT.Next(Ik(k), I(k, s), I(k, s'), CrashTypes.NormalOp(uiop))
   {
     BCS.WriteBackSuperblockStepSyncsGraphs(k, s, s', dop);
-    assert CSBT.NextStep(Ik(k), I(k, s), I(k, s'), uiop, CSBT.SyncStep);
+    assert CSBT.NextStep(Ik(k), I(k, s), I(k, s'), CrashTypes.NormalOp(uiop), CSBT.SyncStep);
   }
 
-  lemma RefinesUnallocStep(k: BBCS.Constants, s: BBCS.Variables, s': BBCS.Variables, uiop: UIOp, dop: DiskOp, ref: Reference)
+  lemma RefinesUnallocStep(k: BBCS.Constants, s: BBCS.Variables, s': BBCS.Variables, uiop: M.UIOp, dop: DiskOp, ref: Reference)
   requires BBCS.Inv(k, s)
   requires BBCS.Inv(k, s')
   requires uiop.NoOp?
   requires BC.Unalloc(k.machine, s.machine, s'.machine, dop, ref)
   requires D.Stutter(k.disk, s.disk, s'.disk, dop);
-  ensures CSBT.Next(Ik(k), I(k, s), I(k, s'), uiop)
+  ensures CSBT.Next(Ik(k), I(k, s), I(k, s'), CrashTypes.NormalOp(uiop))
   {
     BCS.UnallocStepPreservesPersistentGraph(k, s, s', dop, ref);
 
@@ -111,55 +112,55 @@ abstract module BetreeBlockCacheSystemCrashSafeBetreeRefinement {
     DBI.GCStepPreservesInvariant(Ik(k), BBCS.EphemeralBetree(k, s), BBCS.EphemeralBetree(k, s'), iset{ref});
 
     assert BT.NextStep(Ik(k), I(k, s).ephemeral, I(k, s').ephemeral, uiop, BT.GCStep(iset{ref}));
-    assert CSBT.NextStep(Ik(k), I(k, s), I(k, s'), uiop, CSBT.EphemeralMoveStep);
+    assert CSBT.NextStep(Ik(k), I(k, s), I(k, s'), CrashTypes.NormalOp(uiop), CSBT.EphemeralMoveStep);
   }
 
-  lemma RefinesPageInStep(k: BBCS.Constants, s: BBCS.Variables, s': BBCS.Variables, uiop: UIOp, dop: DiskOp, ref: Reference)
+  lemma RefinesPageInStep(k: BBCS.Constants, s: BBCS.Variables, s': BBCS.Variables, uiop: M.UIOp, dop: DiskOp, ref: Reference)
   requires BBCS.Inv(k, s)
   requires BBCS.Inv(k, s')
   requires uiop.NoOp?
   requires BC.PageIn(k.machine, s.machine, s'.machine, dop, ref)
   requires D.Read(k.disk, s.disk, s'.disk, dop);
-  ensures CSBT.Next(Ik(k), I(k, s), I(k, s'), uiop)
+  ensures CSBT.Next(Ik(k), I(k, s), I(k, s'), CrashTypes.NormalOp(uiop))
   {
     BCS.PageInStepPreservesGraphs(k, s, s', dop, ref);
     assert BT.NextStep(Ik(k), I(k, s).ephemeral, I(k, s').ephemeral, uiop, BT.StutterStep);
-    assert CSBT.NextStep(Ik(k), I(k, s), I(k, s'), uiop, CSBT.EphemeralMoveStep);
+    assert CSBT.NextStep(Ik(k), I(k, s), I(k, s'), CrashTypes.NormalOp(uiop), CSBT.EphemeralMoveStep);
   }
 
-  lemma RefinesPageInSuperblockStep(k: BBCS.Constants, s: BBCS.Variables, s': BBCS.Variables, uiop: UIOp, dop: DiskOp)
+  lemma RefinesPageInSuperblockStep(k: BBCS.Constants, s: BBCS.Variables, s': BBCS.Variables, uiop: M.UIOp, dop: DiskOp)
   requires BBCS.Inv(k, s)
   requires BBCS.Inv(k, s')
   requires uiop.NoOp?
   requires BC.PageInSuperblock(k.machine, s.machine, s'.machine, dop)
   requires D.Read(k.disk, s.disk, s'.disk, dop);
-  ensures CSBT.Next(Ik(k), I(k, s), I(k, s'), uiop)
+  ensures CSBT.Next(Ik(k), I(k, s), I(k, s'), CrashTypes.NormalOp(uiop))
   {
     BCS.PageInSuperblockStepPreservesGraphs(k, s, s', dop);
     assert BT.NextStep(Ik(k), I(k, s).ephemeral, I(k, s').ephemeral, uiop, BT.StutterStep);
-    assert CSBT.NextStep(Ik(k), I(k, s), I(k, s'), uiop, CSBT.EphemeralMoveStep);
+    assert CSBT.NextStep(Ik(k), I(k, s), I(k, s'), CrashTypes.NormalOp(uiop), CSBT.EphemeralMoveStep);
   }
 
-  lemma RefinesEvictStep(k: BBCS.Constants, s: BBCS.Variables, s': BBCS.Variables, uiop: UIOp, dop: DiskOp, ref: Reference)
+  lemma RefinesEvictStep(k: BBCS.Constants, s: BBCS.Variables, s': BBCS.Variables, uiop: M.UIOp, dop: DiskOp, ref: Reference)
   requires BBCS.Inv(k, s)
   requires BBCS.Inv(k, s')
   requires uiop.NoOp?
   requires BC.Evict(k.machine, s.machine, s'.machine, dop, ref)
   requires D.Stutter(k.disk, s.disk, s'.disk, dop);
-  ensures CSBT.Next(Ik(k), I(k, s), I(k, s'), uiop)
+  ensures CSBT.Next(Ik(k), I(k, s), I(k, s'), CrashTypes.NormalOp(uiop))
   {
     BCS.EvictStepPreservesGraphs(k, s, s', dop, ref);
     assert BT.NextStep(Ik(k), I(k, s).ephemeral, I(k, s').ephemeral, uiop, BT.StutterStep);
-    assert CSBT.NextStep(Ik(k), I(k, s), I(k, s'), uiop, CSBT.EphemeralMoveStep);
+    assert CSBT.NextStep(Ik(k), I(k, s), I(k, s'), CrashTypes.NormalOp(uiop), CSBT.EphemeralMoveStep);
   }
 
-  lemma RefinesBlockCacheMoveStep(k: BBCS.Constants, s: BBCS.Variables, s': BBCS.Variables, uiop: UIOp, dop: DiskOp, step: BC.Step)
+  lemma RefinesBlockCacheMoveStep(k: BBCS.Constants, s: BBCS.Variables, s': BBCS.Variables, uiop: M.UIOp, dop: DiskOp, step: BC.Step)
   requires BBCS.Inv(k, s)
   requires BBCS.Inv(k, s')
   requires uiop.NoOp?
   requires M.BlockCacheMove(k.machine, s.machine, s'.machine, uiop, dop, step)
   requires D.Next(k.disk, s.disk, s'.disk, dop)
-  ensures CSBT.Next(Ik(k), I(k, s), I(k, s'), uiop)
+  ensures CSBT.Next(Ik(k), I(k, s), I(k, s'), CrashTypes.NormalOp(uiop))
   {
     match step {
       case WriteBackStep(ref) => RefinesWriteBackStep(k, s, s', uiop, dop, ref);
@@ -173,12 +174,12 @@ abstract module BetreeBlockCacheSystemCrashSafeBetreeRefinement {
 
   }
 
-  lemma RefinesMachineStep(k: BBCS.Constants, s: BBCS.Variables, s': BBCS.Variables, uiop: UIOp, dop: DiskOp, step: M.Step)
+  lemma RefinesMachineStep(k: BBCS.Constants, s: BBCS.Variables, s': BBCS.Variables, uiop: M.UIOp, dop: DiskOp, step: M.Step)
   requires BBCS.Inv(k, s)
   requires BBCS.Inv(k, s')
   requires M.NextStep(k.machine, s.machine, s'.machine, uiop, dop, step)
   requires D.Next(k.disk, s.disk, s'.disk, dop)
-  ensures CSBT.Next(Ik(k), I(k, s), I(k, s'), uiop)
+  ensures CSBT.Next(Ik(k), I(k, s), I(k, s'), CrashTypes.NormalOp(uiop))
   {
     match step {
       case BetreeMoveStep(betreeStep) => RefinesBetreeMoveStep(k, s, s', uiop, dop, betreeStep);
@@ -186,18 +187,18 @@ abstract module BetreeBlockCacheSystemCrashSafeBetreeRefinement {
     }
   }
 
-  lemma RefinesMachine(k: BBCS.Constants, s: BBCS.Variables, s': BBCS.Variables, uiop: UIOp, dop: DiskOp)
+  lemma RefinesMachine(k: BBCS.Constants, s: BBCS.Variables, s': BBCS.Variables, uiop: M.UIOp, dop: DiskOp)
   requires BBCS.Inv(k, s)
   requires BBCS.Inv(k, s')
   requires M.Next(k.machine, s.machine, s'.machine, uiop, dop)
   requires D.Next(k.disk, s.disk, s'.disk, dop)
-  ensures CSBT.Next(Ik(k), I(k, s), I(k, s'), uiop)
+  ensures CSBT.Next(Ik(k), I(k, s), I(k, s'), CrashTypes.NormalOp(uiop))
   {
     var step: M.Step :| M.NextStep(k.machine, s.machine, s'.machine, uiop, dop, step);
     RefinesMachineStep(k, s, s', uiop, dop, step);
   }
 
-  lemma RefinesCrash(k: BBCS.Constants, s: BBCS.Variables, s': BBCS.Variables, uiop: UIOp)
+  lemma RefinesCrash(k: BBCS.Constants, s: BBCS.Variables, s': BBCS.Variables, uiop: CrashableUIOp)
   requires BBCS.Inv(k, s)
   requires BBCS.Inv(k, s')
   requires uiop.CrashOp?
@@ -210,7 +211,7 @@ abstract module BetreeBlockCacheSystemCrashSafeBetreeRefinement {
     assert CSBT.NextStep(Ik(k), I(k, s), I(k, s'), uiop, CSBT.CrashStep);
   }
 
-  lemma RefinesNextStep(k: BBCS.Constants, s: BBCS.Variables, s': BBCS.Variables, uiop: UIOp, step: BBCS.Step)
+  lemma RefinesNextStep(k: BBCS.Constants, s: BBCS.Variables, s': BBCS.Variables, uiop: CrashableUIOp, step: BBCS.Step)
   requires BBCS.Inv(k, s)
   requires BBCS.NextStep(k, s, s', uiop, step)
   ensures BBCS.Inv(k, s')
@@ -218,12 +219,12 @@ abstract module BetreeBlockCacheSystemCrashSafeBetreeRefinement {
   {
     BBCS.NextPreservesInv(k, s, s', uiop);
     match step {
-      case MachineStep(dop) => RefinesMachine(k, s, s', uiop, dop);
+      case DamStep(dop) => RefinesMachine(k, s, s', uiop.uiop, dop);
       case CrashStep => RefinesCrash(k, s, s', uiop);
     }
   }
 
-  lemma RefinesNext(k: BBCS.Constants, s: BBCS.Variables, s': BBCS.Variables, uiop: UIOp)
+  lemma RefinesNext(k: BBCS.Constants, s: BBCS.Variables, s': BBCS.Variables, uiop: CrashableUIOp)
   requires BBCS.Inv(k, s)
   requires BBCS.Next(k, s, s', uiop)
   ensures BBCS.Inv(k, s')
